src/coq/Theory/LocalFrame.v
@@ -1,0 +1,407 @@
+From Coq Require Import
+     String Morphisms List.
+
+From ITree Require Import
+     ITree
+     Basics.Monad
+     Eq.Eq
+     TranslateFacts.
+
+From Vellvm Require Import
+     Utils.Tactics
+     Utils.Util
+     Syntax.LLVMAst
+     Syntax.AstLib
+     Syntax.DynamicTypes
+     Syntax.TypToDtyp
+     Semantics.LLVMEvents
+     Semantics.DynamicValues
+     Semantics.TopLevel
+     Semantics.InterpretationStack
+     Handlers.Handlers
+     Refinement
+     Theory.InterpreterCFG
+     Theory.ExpLemmas
+     Theory.InstrLemmas
+     Theory.InterpreterCFG
+     Theory.SymbolicInterpreter.
+
+From ExtLib Require Import
+     Core.RelDec
+     Data.Map.FMapAList
+     Structures.Maps.
+
+From Vellvm Require Import
+     Utils.AListFacts
+     Utils.PostConditions
+     Syntax.Scope.
+
+Import ListNotations.
+Import AlistNotations.
+Import ITreeNotations.
+Import SemNotations.
+
+Definition local_has_changed (l1 : local_env) (defs: list raw_id) : local_env -> Prop :=
+  fun l2 => forall x, ~ In x defs -> l1 @ x = l2 @ x.
+
+Definition lift_pred_L3 (T : Type) (P : local_env -> Prop) :
+  (memory_stack * (local_env * (global_env * T))) -> Prop :=
+  fun '(_,(l,_)) => P l.
+
+Lemma raise_has_all_posts3 : forall {R} s g l m Q,
+    ℑ3 (raise (A := R) s) g l m ⤳ Q.
+Proof.
+  unfold raise; intros.
+  rewrite interp_cfg3_bind.
+  cbn.
+  unfold interp_cfg3.
+  rewrite interp_intrinsics_trigger.
+  cbn.
+  unfold Intrinsics.F_trigger; cbn.
+  rewrite subevent_subevent.
+  rewrite interp_global_trigger; cbn.
+  rewrite subevent_subevent.
+  rewrite interp_local_bind, interp_local_trigger; cbn.
+  rewrite subevent_subevent, bind_bind.
+  rewrite interp_memory_bind, interp_memory_trigger; cbn.
+  rewrite subevent_subevent, !bind_bind.
+  apply has_post_bind; intros [].
+Qed.
+
+Lemma raiseUB_has_all_posts3 : forall {R} s g l m Q,
+    ℑ3 (raiseUB (X := R) s) g l m ⤳ Q.
+Proof.
+  unfold raiseUB; intros.
+  rewrite interp_cfg3_bind.
+  cbn.
+  unfold interp_cfg3.
+  rewrite interp_intrinsics_trigger.
+  cbn.
+  unfold Intrinsics.F_trigger; cbn.
+  rewrite subevent_subevent.
+  rewrite interp_global_trigger; cbn.
+  rewrite subevent_subevent.
+  rewrite interp_local_bind, interp_local_trigger; cbn.
+  rewrite subevent_subevent, bind_bind.
+  rewrite interp_memory_bind, interp_memory_trigger; cbn.
+  rewrite subevent_subevent, !bind_bind.
+  apply has_post_bind; intros [].
+Qed.
+
+Ltac case_eq_id x id :=
+  let EQ := fresh "EQ" in
+  let NEQ := fresh "NEQ" in
+  destruct (Eqv.eqv_dec_p x id) as [EQ | NEQ];
+  [repeat red in EQ; subst | unfold Eqv.eqv, eqv_raw_id in NEQ].
+
+Arguments alist_find : simpl never.
+Hint Unfold In : core.
+
+Lemma pickUnique_is_pure: forall v, pure (ℑ3 (pickUnique v)).
+Proof.
+  unfold pure; intros.
+  unfold pickUnique,concretize_or_pick.
+  break_match_goal.
+  cbn.
+  unfold lift_err.
+  break_match_goal.
+  apply failure_is_pure.
+  vred_C3.
+  apply eutt_Ret; cbn; auto.
+  apply pick_is_pure.
+Qed.
+
+Ltac go := repeat vred_C3. 
+Lemma Intrinsic_preserves_local:
+  forall τ f args g l m,
+    ℑ3 (trigger (Intrinsic τ f args)) g l m ⤳ lift_pred_L3 _ (fun l' => l' = l).
+Proof.
+  intros. unfold ℑ3.
+  rewrite interp_intrinsics_trigger.
+  cbn.
+  break_match_goal.
+  - break_match_goal.
+    + unfold raise.
+      rewrite interp_global_bind.
+      rewrite interp_global_trigger. cbn.
+      rewrite subevent_subevent.
+      rewrite !interp_local_bind.
+      rewrite interp_local_trigger.
+      cbn.
+      rewrite subevent_subevent, !bind_bind.
+      rewrite interp_memory_bind,interp_memory_trigger.
+      cbn.
+      rewrite subevent_subevent, !bind_bind.
+      apply has_post_bind; intros [].
+    + rewrite interp_global_ret, interp_local_ret, interp_memory_ret.
+      apply eutt_Ret; repeat red; auto.
+  - cbn.
+    rewrite subevent_subevent.
+    rewrite interp_global_trigger.
+    cbn; rewrite subevent_subevent.
+    rewrite interp_local_bind, interp_local_trigger.
+    cbn; rewrite subevent_subevent.
+    rewrite !bind_bind.
+    rewrite interp_memory_bind, interp_memory_trigger.
+    destruct m; cbn.
+    break_match_goal.
+    + break_match_goal.
+      * apply has_post_bind; intros [].
+        rewrite interp_memory_bind, interp_memory_ret, bind_ret_l.
+        rewrite interp_local_ret,interp_memory_ret.
+        apply eutt_Ret; repeat red; auto.
+      * rewrite bind_ret_l.
+        rewrite interp_memory_bind, interp_memory_ret, bind_ret_l.
+        rewrite interp_local_ret, interp_memory_ret.
+        apply eutt_Ret; repeat red; auto.
+    + unfold raise; rewrite bind_bind.
+      apply has_post_bind; intros [].
+Qed.
+
+Lemma Call_is_pure:
+  forall τ f args, 
+    pure (ℑ3 (trigger (Call τ f args))). 
+Proof.
+  unfold pure; intros. unfold ℑ3.
+  rewrite interp_intrinsics_trigger.
+  cbn.
+  unfold Intrinsics.E_trigger.
+  rewrite subevent_subevent.
+  rewrite interp_global_trigger.
+  cbn; rewrite subevent_subevent.
+  rewrite interp_local_bind, interp_local_trigger.
+  cbn; rewrite subevent_subevent.
+  rewrite bind_bind.
+  rewrite interp_memory_bind, interp_memory_trigger.
+  cbn; rewrite subevent_subevent.
+  rewrite bind_bind.
+  unfold ReSum_id, id_, Id_IFun.
+  apply has_post_bind; intros.
+  go.
+  rewrite interp_local_ret, interp_memory_ret.
+  apply eutt_Ret; repeat red; auto.
+Qed.
+
+Lemma LocalWrite_local_change :
+  forall id v g l m,
+    ℑ3 (trigger (LocalWrite id v)) g l m
+       ⤳ lift_pred_L3 unit (local_has_changed l [id]).
+Proof.
+  intros.
+  rewrite interp_cfg3_LW.
+  apply eutt_Ret.
+  intros ? NIN. 
+  case_eq_id x id.
+  exfalso; apply NIN; auto. 
+  cbn; rewrite alist_find_neq; auto.
+Qed.
+
+Lemma trigger_Mem_local_change:
+  forall {X : Type} (e : MemoryE X) g l m, 
+    ℑ3 (trigger e: itree instr_E X) g l m ⤳ lift_pred_L3 _ (fun l' => l' = l).
+Proof.
+  intros. unfold ℑ3.
+  rewrite interp_intrinsics_trigger.
+  cbn.
+  rewrite subevent_subevent.
+  rewrite interp_global_trigger.
+  cbn; rewrite subevent_subevent.
+  rewrite interp_local_bind, interp_local_trigger.
+  cbn; rewrite subevent_subevent.
+  rewrite bind_bind.
+  rewrite interp_memory_bind, interp_memory_trigger.
+  cbn.
+  destruct e; cbn.
+  - try (rewrite bind_ret_l, interp_memory_bind, interp_memory_ret, bind_ret_l, interp_local_ret,interp_memory_ret; apply eutt_Ret; red; auto).
+  - unfold lift_pure_err, lift_err.
+    rewrite bind_bind.
+    break_match_goal; [unfold raise; rewrite bind_bind; apply has_post_bind; intros [] |].
+    cbn.
+    try (rewrite ?bind_ret_l, ?interp_memory_bind, ?interp_memory_ret, ?bind_ret_l, interp_local_ret,interp_memory_ret; apply eutt_Ret; red; auto).
+  - unfold lift_pure_err, lift_err.
+    rewrite bind_bind.
+    break_match_goal; [unfold raise; rewrite bind_bind; apply has_post_bind; intros [] |].
+    destruct p; cbn.
+    try (rewrite ?bind_ret_l, ?interp_memory_bind, ?interp_memory_ret, ?bind_ret_l, ?interp_local_ret, ?interp_memory_ret; try apply eutt_Ret; red; auto).
+  - break_match_goal; try (unfold raise; rewrite bind_bind; apply has_post_bind; intros []).
+    break_match_goal; try (unfold raiseUB; rewrite bind_bind; apply has_post_bind; intros []).
+    try (rewrite ?bind_ret_l, ?interp_memory_bind, ?interp_memory_ret, ?bind_ret_l, ?interp_local_ret, ?interp_memory_ret; try apply eutt_Ret; red; auto).
+  - break_match_goal; try (unfold raise; rewrite bind_bind; apply has_post_bind; intros []).
+    try (rewrite ?bind_ret_l, ?interp_memory_bind, ?interp_memory_ret, ?bind_ret_l, ?interp_local_ret, ?interp_memory_ret; try apply eutt_Ret; red; auto).
+  - unfold lift_pure_err, lift_err.
+    rewrite bind_bind.
+    break_match_goal; try (unfold raise; rewrite bind_bind; apply has_post_bind; intros []).
+    cbn; try (rewrite ?bind_ret_l, ?interp_memory_bind, ?interp_memory_ret, ?bind_ret_l, ?interp_local_ret, ?interp_memory_ret; try apply eutt_Ret; red; auto).
+  - break_match_goal; try (unfold raise; rewrite bind_bind; apply has_post_bind; intros []);
+      break_match_goal; try (unfold raise; rewrite bind_bind; apply has_post_bind; intros []); destruct p; cbn.
+    all:try (rewrite ?bind_ret_l, ?interp_memory_bind, ?interp_memory_ret, ?bind_ret_l, ?interp_local_ret, ?interp_memory_ret; try apply eutt_Ret; red; auto).
+  - break_match_goal; try (unfold raise; rewrite bind_bind; apply has_post_bind; intros []).
+    break_match_goal; try (unfold raise; rewrite bind_bind; apply has_post_bind; intros []).
+    break_let.
+    rewrite !bind_bind.
+    unfold lift_undef_or_err.
+    break_match_goal; try (unfold raise; rewrite bind_bind; apply has_post_bind; intros []).
+    break_match_goal; try (unfold raiseUB; rewrite bind_bind; apply has_post_bind; intros []).
+    break_match_goal; try (unfold raise; rewrite bind_bind; apply has_post_bind; intros []).
+    all:try (rewrite ?bind_ret_l, ?interp_memory_bind, ?interp_memory_ret, ?bind_ret_l, ?interp_local_ret, ?interp_memory_ret; try apply eutt_Ret; red; auto).
+Qed.
+
+Lemma Ret_local_change :
+  forall {X : Type} {E} (v : X) g l m,
+    (Ret3 g l m v: itree E _) ⤳ lift_pred_L3 X (local_has_changed l []).
+Proof.
+  intros; apply eutt_Ret; repeat red; auto.
+Qed.
+
+Lemma concretize_or_pick_is_pure : forall v P, pure (ℑ3 (concretize_or_pick v P)).
+Proof.
+  unfold pure; intros.
+  unfold concretize_or_pick.
+  break_match_goal; [| apply pick_is_pure].
+  unfold lift_err.
+  break_match_goal; [apply failure_is_pure |].
+  cbn.
+  go.
+  apply eutt_Ret; cbn; auto.
+Qed.
+
+Ltac __base :=
+  first [apply raise_has_all_posts3 |
+         apply LocalWrite_local_change |
+         apply Ret_local_change | idtac].
+
+Lemma instr_same_local : forall x i g l m,
+    ⟦ (x,i) ⟧i3 g l m ⤳ lift_pred_L3 _ (local_has_changed l (def_sites_instr_id x)). 
+Proof with __base.
+  destruct i; intros.
+  - destruct x; cbn; go...
+  - destruct x; cbn; go... 
+    eapply has_post_bind_strong; [apply expr_are_pure |].
+    intros3; intros (-> & -> & ->).
+    go...
+  - destruct fn,x.
+    + cbn; go.
+      rewrite interp_cfg3_map_monad.
+      apply has_post_bind_strong with (S := lift_state_cfgP (pure_P g l m)).
+      apply map_monad_eutt_state3_ind; [intros [] ? ? ? ? (-> & -> & ->); apply expr_are_pure | cbn; intuition].
+      intros3; intros (-> & -> & ->).
+      break_match_goal.
+      * go.
+        rewrite interp_cfg3_map_monad.
+        apply has_post_bind_strong with (S := lift_state_cfgP (pure_P g l m)).
+        apply map_monad_eutt_state3_ind; [intros [] ? ? ? ? (-> & -> & ->); apply pickUnique_is_pure | cbn; intuition].
+        intros3; intros (-> & -> & ->).
+        unfold ITree.map; go.
+        eapply has_post_bind_strong; [apply Intrinsic_preserves_local |].
+        intros3; intros ->.
+        go...
+      * go.
+        eapply has_post_bind_strong; [apply expr_are_pure |].
+        intros3; intros (-> & -> & ->).
+        eapply has_post_bind_strong; [apply Call_is_pure |].
+        intros3; intros (-> & -> & ->).
+        go...
+    + cbn; go.
+      rewrite interp_cfg3_map_monad.
+      apply has_post_bind_strong with (S := lift_state_cfgP (pure_P g l m)).
+       apply map_monad_eutt_state3_ind; [intros [] ? ? ? ? (-> & -> & ->); apply expr_are_pure | cbn; intuition].
+      intros3; intros (-> & -> & ->).
+      break_match_goal.
+      * go.
+        rewrite interp_cfg3_map_monad.
+        apply has_post_bind_strong with (S := lift_state_cfgP (pure_P g l m)).
+        apply map_monad_eutt_state3_ind; [intros [] ? ? ? ? (-> & -> & ->); apply pickUnique_is_pure | cbn; intuition].
+        intros3; intros (-> & -> & ->).
+        unfold ITree.map; go.
+        eapply has_post_bind_strong; [apply Intrinsic_preserves_local |].
+        intros3; intros ->.
+        go...
+      * go.
+        eapply has_post_bind_strong; [apply expr_are_pure |].
+        intros3; intros (-> & -> & ->).
+        eapply has_post_bind_strong; [apply Call_is_pure |].
+        intros3; intros (-> & -> & ->).
+        go...
+  - destruct x; cbn; go... 
+    eapply has_post_bind_strong; [apply trigger_Mem_local_change |].
+    intros3; intros ->.
+    go...
+  - destruct x, ptr; cbn; go...
+    eapply has_post_bind_strong; [apply expr_are_pure |].
+    intros3; intros (-> & -> & ->).
+    go.
+    eapply has_post_bind_strong; [apply concretize_or_pick_is_pure |].
+    intros3; intros (-> & -> & ->).
+    break_match_goal.
+    all: try (go; eapply has_post_bind_strong; [apply trigger_Mem_local_change | intros3; intros ->]).
+    all: try apply LocalWrite_local_change.
+    apply raiseUB_has_all_posts3.
+  - destruct x, ptr; cbn.
+    __base.
+    destruct val; cbn.
+    go.
+    eapply has_post_bind_strong; [apply expr_are_pure |].
+    intros3; intros (-> & -> & ->).
+    go.
+    eapply has_post_bind_strong; [apply concretize_or_pick_is_pure |].
+    intros3; intros (-> & -> & ->).
+    go.
+    eapply has_post_bind_strong; [apply expr_are_pure |].
+    intros3; intros (-> & -> & ->).
+    go.
+    eapply has_post_bind_strong; [apply pickUnique_is_pure |].
+    intros3; intros (-> & -> & ->).
+    break_match_goal.
+    all: try (eapply has_post_weaken; [apply trigger_Mem_local_change | cbn; intros3; cbn; intros ->; red; auto]).
+    apply raiseUB_has_all_posts3.
+  - cbn; break_match_goal; __base.
+  - cbn; break_match_goal; __base.
+  - cbn; break_match_goal; __base.
+  - cbn; break_match_goal; __base.
+  - cbn; break_match_goal; __base.
+Qed.
+
+Lemma def_sites_code_cons : forall {T} id x i (c : code T),
+    In id (def_sites_code ((x,i):: c))
+    <-> (In id (def_sites_instr_id x) \/ In id (def_sites_code c)).
+Proof.
+  induction c as [| [x' i'] c IH] using rev_ind; cbn.
+  - destruct x; cbn; intuition.
+  - destruct x; cbn; intuition.
+Qed.
+
+Arguments def_sites_code : simpl never.
+
+Lemma local_frame_code : forall c g l m,
+    ⟦ c ⟧c3 g l m ⤳ lift_pred_L3 _ (local_has_changed l (def_sites_code c)).
+Proof.
+  induction c as [| i c IH]; intros.
+  - vred_C3.
+    apply eutt_Ret.
+    intros ? ?; reflexivity.
+  - vred_C3.
+    destruct i as [x i].
+    eapply has_post_bind_strong; [apply instr_same_local |].
+    intros3; cbn; intros H.
+    eapply has_post_weaken.
+    apply IH.
+    intros3; cbn; intros H'.
+    red.
+    intros id NIN.
+    cbn in *.
+    rewrite def_sites_code_cons in NIN.
+    destruct x.
+    + cbn in H.
+      case_eq_id id id0.
+      * exfalso.
+        eapply NIN; cbn; auto. 
+      * replace (l@id) with (l0@id).
+        apply H'.
+        intros abs; apply NIN; auto.
+        symmetry; apply H; auto.
+    + replace (l@id) with (l0@id).
+      apply H'.
+      intros abs; apply NIN; auto.
+      symmetry; apply H; auto.
+Qed.
+
